Reorderings
Signed-off-by: zeramorphic <zeramorphic@proton.me>

ConNF/Counting/OrdSupportEquiv.lean
@@ -1,4 +1,5 @@
 import ConNF.Counting.OrdSupport
+import ConNF.Counting.Reorder
 
 /-!
 # Equivalence of ordered supports
@@ -14,7 +15,67 @@ variable [Params.{u}] {α : Λ} [BasePositions] [FoaAssumptions α] {β : Iic α
 
 namespace OrdSupport
 
-/-- An equivalence of ordered supports.
+/-- Ordered supports are *equivalent* if they are defined on the same set and put support conditions
+in the same order. -/
+structure Equiv (S T : OrdSupport β) : Prop where
+  mem_left (c : SupportCondition β) : c ∈ T → c ∈ S
+  mem_right (c : SupportCondition β) : c ∈ S → c ∈ T
+  lt_iff_lt (c d : SupportCondition β) (hcS : c ∈ S) (hcT : c ∈ T) (hdS : d ∈ S) (hdT : d ∈ T) :
+    (S.cpos c).get hcS < (S.cpos d).get hdS ↔ (T.cpos c).get hcT < (T.cpos d).get hdT
+
+namespace Equiv
+
+def refl (S : OrdSupport β) : Equiv S S where
+  mem_left _ hc := hc
+  mem_right _ hc := hc
+  lt_iff_lt _ _ _ _ _ _ := Iff.rfl
+
+def symm {S T : OrdSupport β} (e : Equiv S T) : Equiv T S where
+  mem_left c hc := e.mem_right c hc
+  mem_right c hc := e.mem_left c hc
+  lt_iff_lt c d hcT hcS hdT hdS := (e.lt_iff_lt c d hcS hcT hdS hdT).symm
+
+def trans {S T U : OrdSupport β} (e : Equiv S T) (f : Equiv T U) : Equiv S U where
+  mem_left c hc := e.mem_left c (f.mem_left c hc)
+  mem_right c hc := f.mem_right c (e.mem_right c hc)
+  lt_iff_lt c d hcS hcU hdS hdU :=
+    (e.lt_iff_lt c d hcS (e.mem_right c hcS) hdS (e.mem_right d hdS)).trans
+    (f.lt_iff_lt c d (f.mem_left c hcU) hcU (f.mem_left d hdU) hdU)
+
+end Equiv
+
+instance setoid (β : Iic α) : Setoid (OrdSupport β) where
+  r S T := Equiv S T
+  iseqv := ⟨Equiv.refl, Equiv.symm, Equiv.trans⟩
+
+theorem mem_iff_mem {S T : OrdSupport β} (h : S ≈ T) (c : SupportCondition β) :
+    c ∈ S ↔ c ∈ T :=
+  ⟨h.mem_right c, h.mem_left c⟩
+
+theorem smul_equiv_smul {S T : OrdSupport β} (h : S ≈ T) (ρ : Allowable β) :
+    ρ • S ≈ ρ • T := by
+  constructor
+  case mem_left =>
+    intro c hc
+    exact h.mem_left (ρ⁻¹ • c) hc
+  case mem_right =>
+    intro c hc
+    exact h.mem_right (ρ⁻¹ • c) hc
+  case lt_iff_lt =>
+    intro c d hcS hcT hdS hdT
+    exact h.lt_iff_lt (ρ⁻¹ • c) (ρ⁻¹ • d) _ _ _ _
+
+end OrdSupport
+
+def OrdSupportClass (β : Iic α) : Type u :=
+  Quotient (OrdSupport.setoid β)
+
+-- TODO: API for `OrdSupportClass` once we know what's needed.
+
+namespace OrdSupport
+
+/--
+`r` is an equivalence of ordered supports `S` and `T`.
 
 Paths in the following diagram starting with `S` or `T` commute, where
 * the morphisms `S ↔ T` are the identity,
@@ -26,83 +87,25 @@ Paths in the following diagram starting with `S` or `T` commute, where
 S ↔ T
 ```
 -/
-@[ext]
-structure Equiv (S T : OrdSupport β) where
-  toFun : μ → μ
-  invFun : μ → μ
-  mem_left (c : SupportCondition β) : c ∈ T → c ∈ S
-  mem_right (c : SupportCondition β) : c ∈ S → c ∈ T
+structure IsEquiv (r : Tree Reorder β) (S T : OrdSupport β) : Prop where
+  equiv : Equiv S T
   toFun_apply (c : SupportCondition β) (hS : c ∈ S) (hT : c ∈ T) :
-    toFun ((S.cpos c).get hS) = (T.cpos c).get hT
+    r c.path ((S.cpos c).get hS) = (T.cpos c).get hT
   invFun_apply (c : SupportCondition β) (hT : c ∈ T) (hS : c ∈ S) :
-    invFun ((T.cpos c).get hT) = (S.cpos c).get hS
-  lt_iff_lt (c d : SupportCondition β) (hcS : c ∈ S) (hcT : c ∈ T) (hdS : d ∈ S) (hdT : d ∈ T) :
-    (S.cpos c).get hcS < (S.cpos d).get hdS ↔ (T.cpos c).get hcT < (T.cpos d).get hdT
+    (r c.path).symm ((T.cpos c).get hT) = (S.cpos c).get hS
 
-namespace Equiv
-
-theorem mem_iff_mem {S T : OrdSupport β} (e : Equiv S T) (c : SupportCondition β) :
-    c ∈ S ↔ c ∈ T :=
-  ⟨e.mem_right c, e.mem_left c⟩
-
-def refl (S : OrdSupport β) : Equiv S S where
-  toFun := id
-  invFun := id
-  mem_left _ hc := hc
-  mem_right _ hc := hc
-  toFun_apply _ _ _ := rfl
-  invFun_apply _ _ _ := rfl
-  lt_iff_lt _ _ _ _ _ _ := Iff.rfl
-
-def symm {S T : OrdSupport β} (e : Equiv S T) : Equiv T S where
-  toFun := e.invFun
-  invFun := e.toFun
-  mem_left c hc := e.mem_right c hc
-  mem_right c hc := e.mem_left c hc
-  toFun_apply c hT hS := e.invFun_apply c hT hS
-  invFun_apply c hS hT := e.toFun_apply c hS hT
-  lt_iff_lt c d hcT hcS hdT hdS := (e.lt_iff_lt c d hcS hcT hdS hdT).symm
-
-def trans {S T U : OrdSupport β} (e : Equiv S T) (f : Equiv T U) : Equiv S U where
-  toFun := f.toFun ∘ e.toFun
-  invFun := e.invFun ∘ f.invFun
-  mem_left c hc := e.mem_left c (f.mem_left c hc)
-  mem_right c hc := f.mem_right c (e.mem_right c hc)
-  toFun_apply c hS hU := by
-    rw [Function.comp_apply, e.toFun_apply c hS (e.mem_right c hS)]
-    exact f.toFun_apply c (e.mem_right c hS) hU
-  invFun_apply c hU hS := by
-    rw [Function.comp_apply, f.invFun_apply c hU (f.mem_left c hU)]
-    exact e.invFun_apply c (f.mem_left c hU) hS
-  lt_iff_lt c d hcS hcU hdS hdU :=
-    (e.lt_iff_lt c d hcS (e.mem_right c hcS) hdS (e.mem_right d hdS)).trans
-    (f.lt_iff_lt c d (f.mem_left c hcU) hcU (f.mem_left d hdU) hdU)
-
-end Equiv
-
-instance setoid (β : Iic α) : Setoid (OrdSupport β) where
-  r S T := Nonempty (Equiv S T)
-  iseqv := by
-    constructor
-    case refl =>
-      intro S
-      exact ⟨Equiv.refl S⟩
-    case symm =>
-      rintro S T ⟨e⟩
-      exact ⟨e.symm⟩
-    case trans =>
-      rintro S T U ⟨e⟩ ⟨f⟩
-      exact ⟨e.trans f⟩
-
-theorem mem_iff_mem_of_equiv {S T : OrdSupport β} (h : S ≈ T) (c : SupportCondition β) :
-    c ∈ S ↔ c ∈ T :=
-  h.some.mem_iff_mem c
+theorem isEquiv_smul {r : Tree Reorder β} {S T : OrdSupport β}
+    (h : IsEquiv r S T) (ρ : Allowable β) :
+    IsEquiv r (ρ • S) (ρ • T) := by
+  constructor
+  case equiv => exact smul_equiv_smul h.equiv ρ
+  case toFun_apply =>
+    intros c hS hT
+    exact h.toFun_apply (ρ⁻¹ • c) hS hT
+  case invFun_apply =>
+    intros c hT hS
+    exact h.invFun_apply (ρ⁻¹ • c) hT hS
 
 end OrdSupport
-
-def OrdSupportClass (β : Iic α) : Type u :=
-  Quotient (OrdSupport.setoid β)
-
--- TODO: API for `OrdSupportClass` once we know what's needed.
 
 end ConNF
