ConNF/Counting.lean
@@ -1,5 +1,7 @@
 import ConNF.Counting.OrdSupport
+import ConNF.Counting.Reorder
 import ConNF.Counting.OrdSupportEquiv
 import ConNF.Counting.CodingFunction
+import ConNF.Counting.CodingFunctionEquiv
 import ConNF.Counting.Spec
 import ConNF.Counting.SpecSame
