ConNF/Counting/CodingFunctionEquiv.lean
@@ -1,0 +1,38 @@
+import ConNF.Counting.CodingFunction
+import ConNF.Counting.OrdSupportEquiv
+
+/-!
+# Equivalences of coding functions
+-/
+
+open MulAction Set Sum
+
+universe u
+
+namespace ConNF
+
+variable [Params.{u}] {α : Λ} [BasePositions] [FoaAssumptions α] {β : Iic α}
+
+namespace CodingFunction
+
+-- TODO: Is this file even needed?
+
+/-- A reordering `r` is an equivalence of coding functions if it is an equivalence of some ordered
+supports in the domains of the coding functions in question. -/
+def IsEquiv (r : Tree Reorder β) (χ₁ χ₂ : CodingFunction β) : Prop :=
+  ∃ S₁ ∈ χ₁, ∃ S₂ ∈ χ₂, OrdSupport.IsEquiv r S₁ S₂
+
+/-- If two coding functions are equivalent, every ordered support in the domain of the first one
+is equivalent to some ordered support in the domain of the second. -/
+def exists_mem_isEquiv {r : Tree Reorder β} {χ₁ χ₂ : CodingFunction β} (h : IsEquiv r χ₁ χ₂)
+    (S₁ : OrdSupport β) (hS₁ : S₁ ∈ χ₁) :
+    ∃ S₂ ∈ χ₂, OrdSupport.IsEquiv r S₁ S₂ := by
+  obtain ⟨T₁, hT₁, T₂, hT₂, h⟩ := h
+  obtain ⟨ρ, rfl⟩ := (χ₁.dom_iff T₁ S₁ hT₁).mp hS₁
+  refine ⟨ρ • T₂, ?_, ?_⟩
+  · exact χ₂.smul_mem ρ hT₂
+  · exact OrdSupport.isEquiv_smul h ρ
+
+end CodingFunction
+
+end ConNF
