ConNF/Counting/Reorder.lean
@@ -1,0 +1,41 @@
+import ConNF.BaseType.Params
+
+universe u
+
+namespace ConNF
+
+variable [Params.{u}]
+
+/-- A reordering of some subset of `μ`.
+Reorders typically have hypotheses attached to them to make them into local order isomorphisms. -/
+structure Reorder where
+  toFun : μ → μ
+  invFun : μ → μ
+
+namespace Reorder
+
+instance : CoeFun Reorder (fun _ => μ → μ) where
+  coe := Reorder.toFun
+
+@[simp]
+theorem toFun_apply (r : Reorder) (ν : μ) :
+    r.toFun ν = r ν :=
+  rfl
+
+def symm (r : Reorder) : Reorder where
+  toFun := r.invFun
+  invFun := r.toFun
+
+@[simp]
+theorem invFun_apply (r : Reorder) (ν : μ) :
+    r.invFun ν = r.symm ν :=
+  rfl
+
+@[simp]
+theorem symm_symm (r : Reorder) :
+    r.symm.symm = r :=
+  rfl
+
+end Reorder
+
+end ConNF
